theories/util/types.v
@@ -398,6 +398,10 @@ Fixpoint big_sepHL2_1 {F G H As Bs} (Φ: ∀A B, F A → G B → H A B → PROP)
   | x +:: xl', y +:: yl', z -:: zl' => Φ _ _ x y z ∗ big_sepHL2_1 Φ xl' yl' zl'
   | _, _, _ => False end%I.
 
+Fixpoint big_sepPLTwo {F G As} (Φ: ∀A, F A → G A → PROP) (xl: plist F As) (yl: plist G As)
+  : PROP := match As, xl, yl with ^[], _, _ => True |
+    _ ^:: _, x -:: xl', y -:: yl' => Φ _ x y ∗ big_sepPLTwo Φ xl' yl' end%I.
+
 End def.
 
 Notation "[∗ hlist] x ∈ xl , P" := (big_sepHL (λ _ x, P%I) xl)
@@ -412,6 +416,10 @@ Notation "[∗ hlist] x ; y ;- z ∈ xl ; yl ;- zl , P" :=
   (big_sepHL2_1 (λ _ _ x y z, P%I) xl yl zl)
   (at level 200, xl, yl, zl at level 10, x, y, z at level 1, right associativity,
     format "[∗  hlist]  x ;  y ;-  z  ∈  xl ;  yl ;-  zl ,  P") : bi_scope.
+
+Notation "[∗ plist] x ; y ∈ xl ; yl , P" := (big_sepPLTwo (λ _ x y, P%I) xl yl)
+  (at level 200, xl, yl at level 10, x, y at level 1, right associativity,
+    format "[∗  plist]  x ;  y  ∈  xl ;  yl ,  P") : bi_scope.
 
 Section lemmas.
 Context `{BiAffine PROP}.
